simplify variable names

BasicLean/Basic.lean
@@ -9,17 +9,19 @@ example : True := True.intro
 
 inductive False : Prop
 
-def False.elim {b : Sort u} (h_False : False) : b :=
-  h_False.rec
+def False.elim {b : Sort u} (false : False) : b :=
+  false.rec
+
+example (false : False): b := False.elim false
 
 def Not (a : Prop) : Prop := a → False
 
-def absurd {a : Prop} {b : Sort v} (h_a : a) (h_Not_a : Not a) : b :=
-  have h_False: False := h_Not_a h_a
-  have res: b := False.elim h_False
+def absurd {a : Prop} {b : Sort v} (ha : a) (Not_a : Not a) : b :=
+  have false: False := Not_a ha
+  have res: b := False.elim false
   res
 
-example (h_p : p) (h_Not_p : Not p) : q := absurd h_p h_Not_p
+example (ha: a) (Not_a : Not a) : b := absurd ha Not_a
 
 def id {α : Sort u} (a : α) : α := a
 
@@ -28,33 +30,41 @@ example : Not False := id
 inductive Eq : α → α → Prop where
   | refl (a : α) : Eq a a
 
-example : Eq p p := Eq.refl p
+example : Eq a a := Eq.refl a
 
 theorem id_eq (a : α) : Eq (id a) a := Eq.refl a
 
+example : Eq (id a) a := id_eq a
+
 theorem eq_id (a : α) : Eq a (id a) := Eq.refl a
 
-abbrev Eq.ndrec.{u1, u2} {α : Sort u2} {a : α} {motive : α → Sort u1} (m : motive a) {b : α} (h : Eq a b) : motive b :=
+example : Eq a (id a) := eq_id a
+
+abbrev Eq.ndrec.{u, v} {α : Sort v} {a : α} {motive : α → Sort u} (m : motive a) {b : α} (h : Eq a b) : motive b :=
   h.rec m
 
-theorem Eq.subst {α : Sort u} {motive : α → Prop} {a b : α} (h₁ : Eq a b) (h₂ : motive a) : motive b :=
-  Eq.ndrec h₂ h₁
+theorem Eq.subst {α : Sort u} {motive : α → Prop} {a b : α} (Eq_ab : Eq a b) (motive_a : motive a) : motive b :=
+  Eq.ndrec motive_a Eq_ab
 
-theorem Eq.symm {α : Sort u} {a b : α} (h_Eq_a_b : Eq a b) : Eq b a :=
-  have h_Eq_a_a: Eq a a := Eq.refl a
-  Eq.subst (motive := fun x => Eq x a) h_Eq_a_b h_Eq_a_a
+theorem Eq.symm {α : Sort u} {a b : α} (Eq_ab : Eq a b) : Eq b a :=
+  have Eq_aa: Eq a a := Eq.refl a
+  Eq.subst (motive := fun x => Eq x a) Eq_ab Eq_aa
 
-theorem Eq.trans {α : Sort u} {a b c : α} (h_Eq_a_b : Eq a b) (h_Eq_b_c : Eq b c) : Eq a c :=
-  Eq.subst (motive := fun x => Eq a x) h_Eq_b_c h_Eq_a_b
+example (Eq_ab: Eq a b): Eq b a := Eq.symm Eq_ab
 
-theorem congrArg {α : Sort u} {β : Sort v} {a₁ a₂ : α} (f : α → β) (h_Eq_a1_a2: Eq a₁ a₂) : Eq (f a₁) (f a₂) :=
-  have h_Eq_f_a1_f_a1: Eq (f a₁) (f a₁) := Eq.refl (f a₁)
-  Eq.subst (motive := fun x => Eq (f a₁) (f x)) h_Eq_a1_a2 h_Eq_f_a1_f_a1
+theorem Eq.trans {α : Sort u} {a b c : α} (Eq_ab : Eq a b) (Eq_bc : Eq b c) : Eq a c :=
+  Eq.subst (motive := fun x => Eq a x) Eq_bc Eq_ab
 
-theorem congrFun {α : Sort u} {β : α → Sort v} {f g : (x : α) → β x} (h_Eq_f_g : Eq f g) (a : α) : Eq (f a) (g a) :=
-  have h_Eq_f_a_f_a : Eq (f a) (f a) := Eq.refl (f a)
-  Eq.subst (motive := fun x => Eq (f a) (x a)) h_Eq_f_g h_Eq_f_a_f_a
+example (Eq_ab : Eq a b) (Eq_bc : Eq b c) : Eq a c := Eq.trans Eq_ab Eq_bc
 
-theorem congr {α : Sort u} {β : Sort v} {f₁ f₂ : α → β} {a₁ a₂ : α} (h_Eq_f1_f2 : Eq f₁ f₂) (h_Eq_a1_a2 : Eq a₁ a₂) : Eq (f₁ a₁) (f₂ a₂) :=
-  have h_Eq_f1_a1_f1_a2 : Eq (f₁ a₁) (f₁ a₂) := congrArg f₁ h_Eq_a1_a2
-  Eq.subst (motive := fun x => Eq (f₁ a₁) (x a₂)) h_Eq_f1_f2 h_Eq_f1_a1_f1_a2
+theorem congrArg {α : Sort u} {β : Sort v} {a b : α} (f : α → β) (Eq_ab: Eq a b) : Eq (f a) (f b) :=
+  have Eq_fa_fa: Eq (f a) (f a) := Eq.refl (f a)
+  Eq.subst (motive := fun x => Eq (f a) (f x)) Eq_ab Eq_fa_fa
+
+theorem congrFun {α : Sort u} {β : α → Sort v} {f g : (x : α) → β x} (Eq_fg : Eq f g) (a : α) : Eq (f a) (g a) :=
+  have Eq_fa_fa : Eq (f a) (f a) := Eq.refl (f a)
+  Eq.subst (motive := fun x => Eq (f a) (x a)) Eq_fg Eq_fa_fa
+
+theorem congr {α : Sort u} {β : Sort v} {f g : α → β} {a b : α} (Eq_fg : Eq f g) (Eq_ab : Eq a b) : Eq (f a) (g b) :=
+  have Eq_fa_fb : Eq (f a) (f b) := congrArg f Eq_ab
+  Eq.subst (motive := fun x => Eq (f a) (x b)) Eq_fg Eq_fa_fb
